<section>
  <title><xref ref="S_cases"></xref></title>
  <subsection>
    <title><xref ref="pr_n-even-odd"></xref></title>
    <p>
      <em>Proposition</em>.
      <em>For each integer <m>n</m>,
      <m>n^2 - 5n + 7</m> is an odd integer</em>.
    </p>
    <proof>
      <p>
        Let <m>n</m> be an integer.
        We will prove that <m>n^2 - 5n + 7</m> is an odd integer by examining the case where <m>n</m> is even and the case where <m>n</m> is odd.
      </p>
      <p>
        In the case where <m>n</m> is even,
        there exists an integer <m>m</m> such that <m>n = 2m</m>.
        So in this case,
        <me>
          \begin{aligned}n^2 - 5n + 7 \amp = \left( 2m \right)^2 - 5 \left( 2m \right) + 7 \\ \amp = 4m^2 - 10m + 6 + 1 \\ \amp = 2 \left(2m^2 - 5m + 3 \right) + 1. \end{aligned}
        </me>
      </p>
      <p>
        Since <m>\left( 2m^2 - 5m + 3 \right)</m> is an integer,
        the last equation shows that if <m>n</m> is even,
        then <m>n^2 - 5n + 7</m> is odd.
      </p>
      <p>
        In the case where <m>n</m> is odd,
        there exists an integer <m>m</m> such that <m>n = 2m +1</m>.
        So in this case,
        <me>
          \begin{aligned}n^2 - 5n + 7 \amp = \left( 2m + 1 \right)^2 - 5 \left( 2m + 1 \right) + 7 \\ \amp = 4m^2 - 6m + 3 \\ \amp = 2 \left(2m^2 - 3m + 1 \right) + 1. \end{aligned}
        </me>
      </p>
      <p>
        Since <m>\left( 2m^2 - 3m + 1 \right)</m> is an integer,
        the last equation shows that if <m>n</m> is odd,
        then <m>n^2 - 5n + 7</m> is odd.
        Hence, by using these two cases,
        we have shown that for each integer <m>n</m>,
        <m>n^2 - 5n + 7</m> is an odd integer.
      </p>
    </proof>
  </subsection>
  <subsection>
    <title><xref ref="pr_absvalue"></xref></title>
    <ol>
      <li>
        <p>
          <m>|4.3| = 4.3</m> and <m>|-\pi| = \pi</m>
        </p>
      </li>
      <li>
        <ol>
          <li>
            <p>
              <m>t = 12</m> or <m>t = -12</m>.
            </p>
          </li>
          <li>
            <p>
              <m>t + 3 = 5</m> or <m>t + 3 = -5</m>.
              So <m>t = 2</m> or <m>t = -8</m>.
            </p>
          </li>
          <li>
            <p>
              <m>t - 4 = \dfrac{1}{5}</m> or <m>t - 4 = -\dfrac{1}{5}</m>.
              So <m>t = \dfrac{21}{5}</m> or <m>t = \dfrac{19}{5}</m>.
            </p>
          </li>
          <li>
            <p>
              <m>3t - 4 = 8</m> or <m>3t - 4 = -8</m>.
              So <m>t = 4</m> or <m>t = -\dfrac{4}{3}</m>.
            </p>
          </li>
        </ol>
      </li>
    </ol>
  </subsection>
</section>