<section>
  <title><xref ref="S_functionsonsets"></xref></title>
  <subsection>
    <title><xref ref="prog_functionsandsets"></xref></title>
    <ol cols="2">
      <li>
        <p>
          <m>f ( A ) = \left\{ s, t \right\}</m>
        </p>
      </li>
      <li>
        <p>
          <m>f ( B ) = \left\{ f ( x ) \mid x \in B \right\} = \left\{ s \right\}</m>
        </p>
      </li>
      <li>
        <p>
          <m>f^{-1} ( C ) = \left\{ x \in S \mid f ( x ) \in C \right\} = \left\{ a, b, c, d \right\}</m>
        </p>
      </li>
      <li>
        <p>
          <m>f^{-1} ( D ) = \left\{ x \in S \mid f ( x ) \in D \right\} = \left\{ a, d \right\}</m>
        </p>
      </li>
    </ol>
  </subsection>
  <subsection>
    <title><xref ref="prog_setsandfunctions"></xref></title>
    <ol>
      <li>
        <p>
          <m>f ( 0 ) = 2</m> <m>f ( 1 ) = 3</m>
          <m>f ( 2 ) = 6</m> <m>f ( 3 ) = 3</m> <m>f ( 4 ) = 2</m>
          <m>f ( 5 ) = 3</m> <m>f ( 6 ) = 6</m> <m>f ( 7 ) = 3</m>
        </p>
      </li>
      <li>
        <ol>
          <li>
            <p>
              <m>f ( A ) = \left\{ 2, 3, 6 \right\}</m> <m>f ( B ) = \left\{ 2, 3, 6 \right\}</m>
              <m>f^{-1} ( C ) = \left\{ 0, 1, 3, 4, 5, 7 \right\}</m> <m>f^{-1} ( D ) = \left\{ 1, 3, 5, 7 \right\}</m>
            </p>
          </li>
        </ol>
      </li>
      <li>
        <ol>
          <li>
            <p>
              <m>f ( A \cap B ) = \left\{ 2 \right\}</m> <m>f ( A ) \cap f ( B ) = \left\{ 2, 3, 6 \right\}</m> So in this case,
              <m>f ( A \cap B ) \subseteq f ( A ) \cap f ( B )</m>.
            </p>
          </li>
          <li>
            <p>
              <m>f ( A ) \cup f ( B ) = \left\{ 2, 3, 6 \right\}</m> <m>f ( A \cup B ) = \left\{ 2, 3, 6 \right\}</m> So in this case,
              <m>f ( A \cup B ) = f ( A ) \cup f ( B )</m>.
            </p>
          </li>
          <li>
            <p>
              <m>f^{-1} ( C ) \cap f^{-1} ( D ) = f^{-1} ( C \cap D ) = \left\{ 1, 3, 5, 7 \right\}</m>.
              So in this case,
              <m>f^{-1} ( C \cap D ) = f^{-1} ( C ) \cap f^{-1} ( D )</m>.
            </p>
          </li>
          <li>
            <p>
              <m>f^{-1} ( C ) \cup f^{-1} ( D ) = f^{-1} ( C \cup D ) = \left\{ 0, 1, 3, 4, 5, 7 \right\}</m>.
              So in this case,
              <m>f^{-1} ( C \cup D ) = f^{-1} ( C ) \cup f^{-1} ( D )</m>.
            </p>
          </li>
        </ol>
      </li>
      <li>
        <p>
          <m>f ( A ) = \left\{ 2, 3, 6 \right\}</m>.
          Hence, <m>f^{-1} \!\left( f ( A ) \right) = \left\{ 0, 1, 2, 3, 4, 5, 6, 7 \right\}</m>.
          So in this case,
          <m>A \subseteq f^{-1} \!\left( f ( A ) \right)</m>.
        </p>
      </li>
      <li>
        <p>
          <m>f^{-1} ( C ) = \left\{ 0, 1, 3, 4, 5, 7 \right\}</m>.
          So <m>f \!\left( f^{-1} ( C ) \right) = \left\{2, 3 \right\}</m>.
          So in this case,
          <m>f \!\left( f^{-1} ( C ) \right) \subseteq C</m>.
        </p>
      </li>
    </ol>
  </subsection>
</section>