<section>
  <title><xref ref="S_recursion"></xref></title>
  <subsection>
    <title><xref ref="prog_thirdfibonacci"></xref></title>
    <proof>
      <p>
        We will use a proof by induction.
        For each natural number <m>n</m>,
        we let <m>P( n )</m> be, <m>f_{3n}</m> is an even natural number.
      </p>
      <p>
        Since <m>f_3 = 2</m>,
        we see that <m>P( 1 )</m> is true and this proves the basis step.
      </p>
      <p>
        For the inductive step,
        we let <m>k</m> be a natural number and assume that <m>P( k )</m> is true.
        That is, assume that <m>f_{3k}</m> is an even natural number.
        This means that there exists an integer <m>m</m> such that
        <men xml:id="eq_progfiba">
          f_{3k}  = 2m
        </men>.
      </p>
      <p>
        We need to prove that <m>P( {k + 1} )</m> is true or that <m>f_{3\left( {k + 1} \right)}</m> is even.
        Notice that <m>3( {k + 1} ) = 3k + 3</m> and,
        hence, <m>f_{3\left( {k + 1} \right)}  = f_{3k + 3}</m>.
        We can now use the recursion formula for the Fibonacci numbers to conclude that
        <me>
          f_{3k + 3}  = f_{3k + 2}  + f_{3k + 1}
        </me>.
      </p>
      <p>
        Using the recursion formula again,
        we get <m>f_{3k + 2}  = f_{3k + 1}  + f_{3k}</m>.
        Putting this all together, we see that
        <md>
          <mrow>f_{3\left( {k + 1} \right)}  \amp = f_{3k + 3}</mrow>
          <mrow>\amp = f_{3k + 2}  + f_{3k + 1}</mrow>
          <mrow>\amp = \left( {f_{3k + 1}  + f_{3k} } \right) + f_{3k + 1}</mrow>
          <mrow xml:id="eq_progfibb">\amp = 2f_{3k + 1}  + f_{3k}</mrow>
        </md>.
      </p>
      <p>
        We now substitute the expression for <m>f_{3k}</m> in equation<nbsp/><xref ref="eq_progfiba"/> into equation<nbsp/><xref ref="eq_progfibb"/>.
        This gives
        <me>
          \begin{aligned}f_{3\left( {k + 1} \right)}  \amp = 2f_{3k + 1}  + 2m \\ f_{3\left( {k + 1} \right)}  \amp = 2\left( {f_{3k + 1}  + m} \right) \end{aligned}
        </me>
      </p>
      <p>
        This preceding equation shows that <m>f_{3\left( {k + 1} \right)}</m> is even.
        Hence it has been proved that if <m>P\left( k \right)</m> is true,
        then <m>P\left( {k + 1} \right)</m> is true and the inductive step has been established.
        By the Principle of Mathematical Induction,
        this proves that for each natural number <m>n</m>,
        the Fibonacci number <m>f_{3n}</m> is an even natural number.
      </p>
    </proof>
  </subsection>
</section>