<section>
  <title><xref ref="S_primefactorizations"></xref></title>
  <subsection>
    <title><xref ref="prog_relativelyprime"></xref></title>
    <ol>
      <li>
        <p>
          If <m>a, p \in \mathbb{Z}</m>, <m>p</m> is prime,
          and <m>p</m> divides <m>a</m>,
          then <m>\gcd ( {a, p} ) = p</m>.
        </p>
      </li>
      <li>
        <p>
          If <m>a, p \in \mathbb{Z}</m>, <m>p</m> is prime,
          and <m>p</m> does not divide <m>a</m>,
          then <m>\gcd ( {a, p} ) = 1</m>.
        </p>
      </li>
      <li>
        <p>
          Three examples are <m>\gcd ( {4, 9} ) = 1</m>,
          <m>\gcd ( {15, 16} ) = 1</m>,
          <m>\gcd ( {8, 25} ) = 1</m>.
        </p>
      </li>
    </ol>
  </subsection>
  <subsection>
    <title><xref ref="prog_relativelyprimeprop"></xref></title>
    <p>
      <em><xref ref="T_relativelyprimeprop">Theorem</xref></em>.
      Let <m>a</m>, <m>b</m>, and <m>c</m> be integers.
      If <m>a</m> and <m>b</m> are relatively prime and
      <m>a \mid ( {bc} )</m>, then <m>a \mid c</m>.
    </p>
    <proof>
      <p>
        Let <m>a</m>, <m>b</m>, and <m>c</m> be integers.
        Assume that <m>a</m> and <m>b</m> are relatively prime and <m>a \mid ( {bc} )</m>.
        We will prove that <m>a</m> divides <m>c</m>.
      </p>
      <p>
        Since <m>a</m> divides <m>bc</m>,
        there exists an integer <m>k</m> such that
        <men xml:id="eq_814a">
          bc = ak
        </men>.
      </p>
      <p>
        In addition,
        we are assuming that <m>a</m> and <m>b</m> are relatively prime and hence <m>\gcd ( {a, b} ) = 1</m>.
        So by <xref ref="T_gcddivideslincombs">Theorem</xref>,
        there exist integers <m>m</m> and <m>n</m> such that
        <men xml:id="eq_814b">
          am + bn = 1
        </men>.
      </p>
      <p>
        We now multiply both sides of equation<nbsp/><xref ref="eq_814b"/> by <m>c</m>.
        This gives
        <md>
          <mrow>( {am + bn} )c \amp = 1 \cdot c</mrow>
          <mrow xml:id="eq_814c">acm + bcn \amp = c</mrow>
        </md>
      </p>
      <p>
        We can now use equation<nbsp/><xref ref="eq_814a"/> to substitute <m>bc = ak</m> in equation<nbsp/><xref ref="eq_814c"/> and obtain
        <me>
          acm + akn = c
        </me>.
      </p>
      <p>
        If we now factor the left side of this last equation,
        we see that <m>a( {cm + kn} ) = c</m>.
        Since <m>( {cm + kn} )</m> is an integer,
        this proves that <m>a</m> divides <m>c</m>.
        Hence, we have proven that if <m>a</m> and <m>b</m> are relatively prime and
        <m>a \mid ( {bc} )</m>, then <m>a \mid c</m>.
      </p>
    </proof>
  </subsection>
</section>