<section>
  <title><xref ref="S_directproof"></xref></title>
  <ul>
    {{ <xref ref="exer_sec31-prove"></xref>.}}
    \item
    <ul>
      {{(a)}}
      \item Since <m>a \mid b</m> and <m>a \mid c</m>, there exist integers <m>m</m> and <m>n</m> such that <m>b = am</m> and <m>c = an</m>.  Hence,
      <md>
        <mrow>b - c \amp = am - an</mrow>
        <mrow>\amp = a(m - n)</mrow>
      </md>
      Since <m>m - n</m> is an integer (by the closure properties of the integers), the last equation implies that <m>a</m> divides <m>b - c</m>.
    </ul>
  </ul>
  <ul>
    \item
    <ul>
      {{(b)}}
      \item What do you need to do in order to prove that <m>n^3</m> is odd?  Notice that if <m>n</m> is an odd integer, then there exists an integer <m>k</m> such that <m>n = 2k + 1</m>.  Remember that to prove that <m>n^3</m> is an odd integer, you need to prove that there exists an integer <m>q</m> such that <m>n^3 = 2q + 1</m>.
      This can also be approached as follows:  If <m>n</m> is odd, then  by <xref ref="T_xyodd"></xref>, <m>n^2</m> is odd.  Now use the fact that <m>n^3 = n \cdot n^2</m>.
    </ul>
  </ul>
  <ul>
    \item
    <ul>
      {{(c)}}
      \item If 4 divides <m>(a - 1)</m>, then there exists an integer <m>k</m> such that <m>a - 1 = 4k</m> and so
      <m>a = 4k + 1</m>.  Use algebra to rewrite <m>\left( a^2 - 1 \right) = (4k + 1)^2 - 1</m>.
    </ul>
  </ul>
  <ul>
    {{2.}}
    \item
    <ol>
      <li>
        <p>
          The natural number <m>n = 9</m> is a counterexample since <m>n</m> is odd,
          <m>n > 3</m>, <m>n^2 - 1 = 80</m> and 3 does not divide 80.
        </p>
      </li>
      <li>
        <p>
          The integer <m>a = 3</m> is a counterexample since
          <m>a^2 - 1 = 8</m> and <m>a - 1 = 2</m>.
          Since 4 divides 8 and 4 does not divide 2, this is an example where the hypothesis of the conditional statement is true and the conclusion is false.
        </p>
      </li>
    </ol>
  </ul>
  <ul>
    {{ <xref ref="exer_3truefalse"></xref>.}}
    \item
    <ol>
      <li>
        <p>
          This statement is false.
          One counterexample is <m>a = 3</m> and <m>b = 2</m> since this is an example where the hypothesis is true and the conclusion is false.
        </p>
      </li>
      <li>
        <p>
          This statement is false.
          One counterexample is <m>n = 5</m>.
          Since <m>n^2 - 4 = 21</m> and <m>n - 2 = 3</m>,
          this is an example where the hypothesis of the conditional statement is true and the conclusion is false.
        </p>
      </li>
      <li>
        <p>
          Make sure you first try some examples.
          How do you prove that an integer is an odd integer?
        </p>
      </li>
      <li>
        <p>
          The following algebra may be useful.
          <me>
            4 \left( 2m + 1 \right)^2 + 7 \left( 2m + 1 \right) + 6 = 16m^2 + 30m + 17
          </me>.
        </p>
      </li>
      <li>
        <p>
          This statement is false.
          One counterexample is <m>a = 7</m>,
          <m>b = 1</m>, and <m>d = 2</m>.
          Why is this a counterexample?
        </p>
      </li>
    </ol>
  </ul>
  <ul>
    {{ <xref ref="exer_diveach"></xref>.}}
    \item
    <ul>
      {{(a)}}
      \item If <m>xy = 1</m>, then <m>x</m> and <m>y</m> are both divisors of <m>1</m>, and the only divisors of <m>1</m> are <m>-1</m> and <m>1</m>.
    </ul>
  </ul>
  <ul>
    \item
    <ul>
      {{(b)}}
      \item Part<nbsp/>(a) is useful in proving this.
    </ul>
  </ul>
  <ul>
    {{ <xref ref="exer_sec31-10"></xref>.}}
    \item <em>Another hint</em>:  <m>\left( 4n + 3 \right) - 2 \left( 2n + 1 \right) = 1</m>.
  </ul>
  <ul>
    {{ <xref ref="exer_congmod3"></xref>.}}
    \item Assuming <m>a</m> and <m>b</m> are both congruent to 2 modulo 3, there exist integers <m>m</m> and <m>n</m> such that <m>a = 3m + 2</m> and <m>b = 3n + 2</m>.
    For part<nbsp/>(a), show that
    <me>
      a + b - 1 = 3 \left( m + n + 1 \right)
    </me>.
    We can then conclude that 3 divides <m>(a + b) - 1</m> and this proves that <m>\mod{a+b}{1}{3}</m>.
    For part<nbsp/>(b), show that
    <me>
      a \cdot b - 1 = 3(3mn + 2m + 2n + 1)
    </me>.
    We can then conclude that 3 divides <m>a \cdot b- 1</m> and this proves that <m>\mod{a \cdot b}{1}{3}</m>.
  </ul>
  <ul>
    {{ <xref ref="exer_cong-props"></xref>.}}
    \item
    <ul>
      <li>
        <title>(a)</title>
        <p>
          Let <m>n \in \N</m>.
          If <m>a</m> is an integer, then
          <m>a - a = 0</m> and <m>n</m> divides 0.
          Therefore, <m>\mod{a}{a}{n}</m>.
        </p>
      </li>
      <li>
        <title>(b)</title>
        <p>
          Let <m>n \in \mathbb{N}</m>, let
          <m>a,
          b \in \mathbb{Z}</m> and assume that <m>\mod{a}{b}{n}</m>.
          We will prove that <m>\mod{b}{a}{n}</m>.
          Since <m>\mod{a}{b}{n}</m>,
          <m>n</m> divides <m>(a - b)</m> and so there exists an integer <m>k</m> such that <m>a - b = nk</m>.
          From this, we can show that
          <m>b - a = n(-k)</m> and so <m>n</m> divides <m>(b - a)</m>.
          Hence, if <m>\mod{a}{b}{n}</m>,
          then <m>\mod{b}{a}{n}</m>.
        </p>
      </li>
    </ul>
  </ul>
  <ul>
    {{ <xref ref="exer_sec31-11"></xref>.}}
    \item The assumptions mean that <m>n \mid \left( a-b \right)</m> and that
    <m>n \mid \left( c-d \right)</m>.  Use these divisibility relations to obtain an expression that is equal to  <m>a</m>  and to obtain an expression that is equal to  <m>c</m>.  Then use algebra to rewrite the resulting expressions for <m>a + c</m>    and <m>a \cdot c</m>.
  </ul>
</section>