<section>
  <title><xref ref="S_inversefunctions"></xref></title>
  <ul>
    {{ <xref ref="exer_sec65-2"></xref>.}}
    \item
    <ul>
      {{(b)}}
      \item <m>f^{ - 1}  = \left\{ {( {c,a} ),( {b,b} ),( {d,c} ),( {a,d} )} \right\}</m>
    </ul>
  </ul>
  <ul>
    \item
    <ul>
      {{(d)}}
      \item For each <m>x \in S</m>, <m>\left( {f^{ - 1}  \circ f} \right)( x ) = x = ( {f \circ f^{ - 1} } )( x )</m>.  This illustrates
      <xref ref="C_inversecomposition">Corollary</xref>.
    </ul>
  </ul>
  <ul>
    {{ <xref ref="exer_solveequation"></xref>.}}
    \item
    <ol>
      <li>
        <p>
          This is a use of <xref ref="C_inversecomposition">Corollary</xref>
          since the cube root function and the cubing function are inverse functions of each other and consequently,
          the composition of the cubing function with the cube root function is the identity function.
        </p>
      </li>
      <li>
        <p>
          This is a use of <xref ref="C_inversecomposition">Corollary</xref>
          since the natural logarithm function and the exponential function with base <m>e</m> are inverse functions of each other and consequently,
          the composition of the natural logarithm function with the exponential function with base <m>e</m> is the identity function.
        </p>
      </li>
      <li>
        <p>
          They are similar because they both use the concept of an inverse function to
          <q>undo</q>
          one side of the equation.
        </p>
      </li>
    </ol>
  </ul>
  <ul>
    {{ <xref ref="exer_inversecomposition"></xref>.}}
    \item Using the notation from <xref ref="C_inversecomposition">Corollary</xref>, if <m>y = f(x)</m> and
    <m>x = f^{-1}(y)</m>, then
    <md>
      <mrow>\left(f \circ f^{-1} \right) (y) \amp = f ( f^{-1} ( y ) )</mrow>
      <mrow>\amp = f ( x )</mrow>
      <mrow>\amp = y</mrow>
    </md>
  </ul>
  <ul>
    {{ <xref ref="exer_compequalidentity"></xref>.}}
    \item
    <ul>
      {{(a)}}
      \item Let <m>x, y \in A</m> and assume that
      <m>f ( x ) = f ( y )</m>.  Apply <m>g</m> to both sides of this equation to prove that
      <m>( g \circ f ) ( x ) = ( g \circ f ) ( y )</m>.
      Since <m>g \circ f = I_A</m>, this implies that <m>x = y</m> and hence that <m>f</m> is an injection.
    </ul>
  </ul>
  <ul>
    \item
    <ul>
      {{(b)}}
      \item Start by assuming that <m>f \circ g = I_B</m>, and then let <m>y \in B</m>.  You need to prove there exists an <m>x \in A</m> such that <m>f ( x ) = y</m>.
    </ul>
  </ul>
  <ul>
    {{ <xref ref="exer_sec65-6"></xref>.}}
    \item
    <ol>
      <li>
        <p>
          <m>f:\mathbb{R} \to \mathbb{R}</m> is defined by <m>f\left( x \right) = e^{ - x^2 }</m>.
          Since this function is not an injection,
          the inverse of <m>f</m> is not a function.
        </p>
      </li>
      <li>
        <p>
          <m>g:\mathbb{R}^* \to \left( {0, 1} \right]</m> is defined by <m>g\left( x \right) = e^{ - x^2 }</m>.
          In this case, <m>g</m> is a bijection and hence,
          the inverse of <m>g</m> is a function.
          To see that <m>g</m> is an injection, assume that
          <m>x,
          y \in \mathbb{R}^*</m> and that <m>e^{-x^2} = e^{-y^2}</m>.
          Then, <m>x^2 = y^2</m> and since
          <m>x,
          y \geq 0</m>, we see that <m>x = y</m>.
          To see that <m>g</m> is a surjection,
          let <m>y \in \left( 0, 1 \right]</m>.
          Then, <m>\ln y \lt 0</m> and <m>- \ln y > 0</m>,
          and <m>g \left( \sqrt{-\ln y} \right) = y</m>.
        </p>
      </li>
    </ol>
  </ul>
</section>