<section>
  <title><xref ref="S_moremethods"></xref></title>
  <ul>
    {{ <xref ref="exer_ncubed"></xref>.}}
    \item
    <ul>
      {{(a)}}
      \item Let  <m>n</m>  be an even integer.  Since  <m>n</m>  is even, there exists an integer  <m>k</m> such that
      <m>n = 2k</m>. Now use this to prove that <m>n^3</m>   must be even.
    </ul>
  </ul>
  <ul>
    \item
    <ul>
      {{(b)}}
      \item Prove the contrapositive.
    </ul>
  </ul>
  <ul>
    \item
    <ul>
      {{(c)}}
      \item Explain why Parts (a) and (b) prove this.
    </ul>
  </ul>
  <ul>
    \item
    <ul>
      {{(d)}}
      \item Explain why Parts (a) and (b) prove this.
    </ul>
  </ul>
  <ul>
    {{ <xref ref="exer_sec32-2"></xref>.}}
    \item
    <ul>
      {{(a)}}
      \item The contrapositive is,  For all integers <m>a</m>  and  <m>b</m>, if  <m>\mod{ab}{0}{6}</m>,
      then  <m>\mod{a}{0}{6}</m>  or   <m>\mod{b}{0}{6}</m>.
    </ul>
  </ul>
  <ul>
    {{3}.}
    \item
    <ol>
      <li>
        <p>
          The contrapositive is: For all positive real numbers <m>a</m> and <m>b</m>,
          if <m>a = b</m>, then <m>\sqrt{ab} = \dfrac{a + b}{2}</m>.
        </p>
      </li>
      <li>
        <p>
          The statement is true.
          If <m>a = b</m>, then <m>\dfrac{a + b}{2} = \dfrac{2a}{2} = a</m>,
          and <m>\sqrt{ab} = \sqrt{a^2} = a</m>.
          This proves the contrapositive.
        </p>
      </li>
    </ol>
  </ul>
  <ul>
    {{ <xref ref="exer_sec32-4"></xref>.}}
    \item
    <ol>
      <li>
        <p>
          True.
          If <m>a \equiv 2 \pmod 5</m>,
          then there exists an integer <m>k</m> such that <m>a - 2 = 5k</m>.
          Then,
          <me>
            a^2 - 4  = \left( 2 + 5k \right)^2 - 4  = 20k + 25k^2
          </me>.
          This means that <m>a^2 - 4 = 5 \left( 4k + 5k^2 \right)</m>,
          and hence, <m>a^2 \equiv 4 \pmod 5</m>.
        </p>
      </li>
      <li>
        <p>
          False.
          A counterexample is <m>a = 3</m> since
          <m>\mod{3^2}{4}{5}</m> and <m>\notmod{3}{2}{5}</m>.
        </p>
      </li>
      <li>
        <p>
          False.
          Part<nbsp/>(b) shows this is false.
        </p>
      </li>
    </ol>
  </ul>
  <ul>
    {{ <xref ref="exer_sec32-congmod7"></xref>.}}
    \item
    <ol>
      <li>
        <p>
          For each integer <m>a</m>, if <m>a \equiv 3 \pmod 7</m>,
          then <m>(a^2 + 5a) \equiv 3 \pmod 7</m>,
          and for each integer <m>a</m>,
          if <m>(a^2 + 5a) \equiv 3 \pmod 7</m>,
          then <m>a \equiv 3 \pmod 7</m>.
        </p>
      </li>
      <li>
        <p>
          For each integer <m>a</m>,
          if <m>a \equiv 3 \pmod 7</m>,
          then <m>(a^2 + 5a) \equiv 3 \pmod 7</m> is true.
          To prove this, if <m>a \equiv 3 \pmod 7</m>,
          then there exists an integer <m>k</m> such that <m>a = 3 + 7k</m>.
          We can then prove that
          <me>
            \left( a^2 + 5a \right) - 3 = 21 + 77k + 49k^2 = 7(3 + 11k + 7k^2)
          </me>.
          This shows that <m>(a^2 + 5a) \equiv 3 \pmod 7</m>.
          For each integer <m>a</m>,
          if <m>(a^2 + 5a) \equiv 3 \pmod 7</m>,
          then <m>a \equiv 3 \pmod 7</m> is false.
          A counterexample is <m>a = 6</m>.
          When <m>a = 6</m>, <m>a^2 + 5a = 66</m> and
          <m>66 \equiv 3 \pmod 7</m> and <m>6 \not \equiv 3 \pmod 7</m>.
        </p>
      </li>
      <li>
        <p>
          Since one of the two conditional statements in Part<nbsp/>(b) is false,
          the given proposition is false.
        </p>
      </li>
    </ol>
  </ul>
  <ul>
    {{ <xref ref="exer_sec32-6"></xref>.}}
    \item Prove both of the conditional statements:  (1) If the area of the right triangle is
    <m>c^2/4</m>, then the right triangle is an isosceles triangle.  (2)  If the right triangle is an isosceles triange, then the area of the right triangle is <m>c^2/4</m>.
  </ul>
  <ul>
    {{ <xref ref="exer_sec32-rational"></xref>.}}
    \item The statement is true.  It is easier to prove the contrapositive, which is:
    <ul>
      \item For each positive real number <m>x</m>, if <m>\sqrt{x}</m> is rational, then <m>x</m> is rational.
    </ul>
    Let <m>x</m> be a positive real number.  If there exist positive integers <m>m</m> and <m>n</m> such that <m>\sqrt{x} = \dfrac{m}{n}</m>, then
    <m>x = \dfrac{m^2}{n^2}</m>.
  </ul>
  <ul>
    {{ <xref ref="exer_sec32-8"></xref>.}}
    \item Remember that there are two conditional statements associated with this biconditional statement.  Be willing to consider the contrapositive of one of these conditional statements.
  </ul>
  <ul>
    {{ <xref ref="exer_IVT"></xref>.}}
    \item Define an appropriate function and use the Intermediate Value Theorem.
  </ul>
  <ul>
    {{ <xref ref="exer_sec32-16"></xref>.}}
    \item
    <ul>
      {{(b)}}
      \item Since 4 divides <m>a</m>, there exist an integer <m>n</m> such that <m>a = 4n</m>.  Using this, we see that <m>b^3 = 16n^2</m>. This means that <m>b^3</m> is even and hence by Exercise<nbsp/>(1), <m>b</m> is even.   So there exists an integer <m>m</m> such that <m>b = 2m</m>.  Use this to prove that <m>m^3</m> must be even and hence by Exercise<nbsp/>(1), <m>m</m> is even.
    </ul>
  </ul>
  <ul>
    {{ <xref ref="exer_sec32-equation17"></xref>.}}
    \item It may be necessary to factor a sum  of cubes.  Recall that
    <me>
      u^3 + v^3 = ( u + v ) ( u^2 - uv + v^2 )
    </me>.
  </ul>
</section>