<section>
  <title><xref ref="S_logequiv"></xref></title>
  <subsection>
    <title><xref ref="pr_workingeq2"></xref></title>
    <ol>
      <li>
        <p>
          Starting with the suggested equivalency, we obtain
          <md>
            <mrow>\left( {P \wedge \mynot  Q} \right) \to R \amp \equiv \mynot \left( P \wedge \mynot Q \right) \vee R</mrow>
            <mrow>\amp \equiv \left( \mynot P \vee \mynot \left( \mynot Q \right) \right) \vee R</mrow>
            <mrow>\amp \equiv \mynot P \vee \left( Q \vee R \right)</mrow>
            <mrow>\amp \equiv P \to \left( Q \vee R \right)</mrow>
          </md>
        </p>
      </li>
      <li>
        <p>
          For this, let <m>P</m> be,
          <q>3 is a factor of <m>a \cdot b</m>,</q>
          let <m>Q</m> be,
          <q>3 is a factor of <m>a</m>,</q>
          and let <m>R</m> be,
          <q>3 is a factor of <m>b</m>.</q>
          Then the stated proposition is written in the form <m>P \to \left( {Q \vee R} \right)</m>.
          Since this is logically equivalent to <m>\left( {P \wedge \mynot Q} \right) \to R</m>,
          if we prove that if 3 is a factor of
          <m>a \cdot b</m> and 3 is not a factor of <m>a</m>,
          then 3 is a factor of <m>b</m>,
          then we have proven the original proposition.
        </p>
      </li>
    </ol>
  </subsection>
</section>