<section>
  <title><xref ref="S_moremethods"></xref></title>
  <subsection>
    <title><xref ref="pr_contrapositive"></xref></title>
    <ol>
      <li>
        <p>
          For all real numbers <m>a</m> and <m>b</m>,
          if <m>ab = 0</m>, then <m>a = 0\text{ or } b = 0</m>.
        </p>
      </li>
      <li>
        <p>
          For all real numbers <m>a</m> and <m>b</m>,
          if <m>ab = 0</m> and <m>a \ne 0</m>, <m>b = 0</m>.
        </p>
      </li>
      <li>
        <p>
          This gives
          <me>
            \frac{1}{a} (ab) = \frac{1}{a} \cdot 0
          </me>.
          We now use the associative property on the left side of this equation and simplify both sides of the equation to obtain
          <md>
            <mrow>\left( \frac{1}{a} \cdot a \right)b \amp = 0</mrow>
            <mrow>1 \cdot b \amp = 0</mrow>
            <mrow>b \amp = 0</mrow>
          </md>
          Therefore, <m>b = 0</m> and this completes the proof of a statement that is logically equivalent to the contrapositive.
          Hence, we have proved the proposition.
        </p>
      </li>
    </ol>
  </subsection>
</section>