<section>
  <title><xref ref="S_moreaboutfunctions"></xref></title>
  <ul>
    {{ <xref ref="exer_sec62-1"></xref>.}}
    \item
    <ul>
      {{(a)}}
      \item <m>f( 0 ) = 4</m>, <m>f( 1 ) = 0, f( 2 ) = 3</m>,
      <m>f( 3 ) = 3</m>, <m>f( 4 ) = 0</m>
    </ul>
  </ul>
  <ul>
    \item
    <ul>
      {{(b)}}
      \item <m>g( 0 ) = 4</m>, <m>g( 1 ) = 0, g( 2 ) = 3</m>,
      <m>g( 3 ) = 3</m>, <m>g( 4 ) = 0</m>
    </ul>
  </ul>
  <ul>
    \item
    <ul>
      {{(c)}}
      \item The two functions are equal.
    </ul>
  </ul>
  <ul>
    {{ <xref ref="exer62_realfunction"></xref>.}}
    \item
    <ol>
      <li>
        <p>
          <m>f(2) = 9</m>, <m>f(-2) = 9</m>,
          <m>f(3) = 14</m>, <m>f(\sqrt{2} = 7</m>
        </p>
      </li>
      <li>
        <p>
          <m>g(0) = 5</m>, <m>g(2) = 9</m>,
          <m>g(-2) = 9</m>, <m>g(3) = 14</m>, <m>g(\sqrt{2}) = 7</m>
        </p>
      </li>
      <li>
        <p>
          The function <m>f</m> is not equal to the function <m>g</m> since they do not have the same domain.
        </p>
      </li>
      <li>
        <p>
          The function <m>h</m> is equal to the function <m>f</m> since if <m>x \ne 0</m>,
          then <m>\dfrac{x^2 + 5x}{x} = x^2 + 5</m>.
        </p>
      </li>
    </ol>
  </ul>
  <ul>
    {{ <xref ref="exer_sec62-3"></xref>.}}
    \item
    <ul>
      {{(a)}}
      \item <m>\left\langle {a_n } \right\rangle</m>,  where  <m>a_n  = \dfrac{1}{{n^2 }}</m>  for each
      <m>n \in \mathbb{N}</m>.  The domain is  <m>\mathbb{N}</m>, and <m>\Q</m> can be the codomain.
    </ul>
  </ul>
  <ul>
    \item
    <ul>
      {{(d)}}
      \item <m>\left\langle {a_n } \right\rangle</m>,  where  <m>a_n  = \cos ( {n\pi } )</m>  for each  <m>n \in \mathbb{N} \cup {0}</m>.  The domain is  <m>\mathbb{N} \cup {0}</m>, and <m>\left\{ -1, 1 \right\}</m> can be the codomain.  This sequence is equal to the sequence in Part<nbsp/>(c).
    </ul>
  </ul>
  <ul>
    {{ <xref ref="sym_projfunc"></xref>.}}
    \item
    <ul>
      {{(a)}}
      \item <m>p_1(1, x) = 1</m>, <m>p_1(1, y) = 1</m>, <m>p_1(1, z) = 1</m>, <m>p_1(2, x) = 2</m>, <m>p_1(2, y) = 2</m>,
      <m>p_1(2, z) = 2</m>
    </ul>
  </ul>
  <ul>
    \item
    <ul>
      {{(c)}}
      \item <m>\text{ range } ( p_1 ) = A</m>, <m>\text{ range } ( p_2 ) = B</m>
    </ul>
  </ul>
  <ul>
    {{ <xref ref="exer_sec62-6"></xref>.}}
    \item Start of the inductive step:  Let <m>P ( n )</m> be
    <q>A convex polygon with <m>n</m> sides has <m>\dfrac{n ( n-3 )}{2}</m> diagonals.</q>
    Let  <m>k \in D</m>  and assume that <m>P ( k )</m> is true, that is, a convex polygon with  <m>k</m>  sides has  <m>\dfrac{{k( {k - 3} )}}{2}</m>  diagonals.   Now let  <m>Q</m>  be convex polygon with  <m>( {k + 1} )</m> sides.  Let  <m>v</m>  be one of the <m>( {k + 1} )</m> vertices of <m>Q</m>  and let  <m>u</m>  and  <m>w</m>  be the two vertices adjacent to  <m>v</m>.  By drawing the line segment from  <m>u</m>  to  <m>w</m> and omitting the vertex  <m>v</m>, we form a convex polygon with  <m>k</m>  sides.  Now complete the inductive step.
  </ul>
  <ul>
    {{ <xref ref="exer_sec61-7"></xref>.}}
    \item
    <ul>
      {{(a)}}
      \item <m>f( { - 3, 4} ) = 9</m>, <m>f( { - 2, - 7} ) =  - 23</m>
    </ul>
  </ul>
  <ul>
    \item
    <ul>
      {{(b)}}
      \item <m>\text{ range } (f) = \left\{ { {( {m, n} ) \in \mathbb{Z} \times \mathbb{Z} } \mid m = 4 - 3n} \right\}</m>
    </ul>
  </ul>
  <ul>
    {{ <xref ref="exer_sec61-8"></xref>.}}
    \item
    <ol>
      <li>
        <p>
          <m>g ( 3, 5 ) = ( 6, -2 )</m>,
          <m>g ( -1, 4 ) = ( -2, -5 )</m>.
        </p>
      </li>
      <li>
        <p>
          The set of preimages of <m>( 8, -3 )</m> is <m>\left\{ ( 4, 7 ) \right\}</m>.
        </p>
      </li>
    </ol>
  </ul>
  <ul>
    {{ <xref ref="exer_determinant"></xref>.}}
    \item
    <ul>
      {{(a)}}
      \item <m>\det \left[ {\begin{array}{*{20}c}
      3 \amp  5  \\
      4 \amp  1
      \end{array}  } \right] =  - 17, \det \left[ {\begin{array}{*{20}c}
      1 \amp  0  \\
      0 \amp  7
      \end{array}  } \right] = 7, \text{ and det } \left[ {\begin{array}{*{20}c}
      3 \amp  { - 2}  \\
      5 \amp  0
      \end{array}  } \right] = 10</m>
    </ul>
  </ul>
</section>