<section>
  <title><xref ref="S_cases"></xref></title>
  <ul>
    {{ <xref ref="exer_consecutive"></xref>.}}
    \item Use the fact that <m>n^2 + n = n ( n+1 )</m>.
  </ul>
  <ul>
    {{ <xref ref="exer_sec33-6"></xref>.}}
    \item Do not use the quadratic formula.  Try a proof by contradiction.  If there exists a  solution of the equation <m>x^2 + x - u = 0</m> that is an integer, then we can conclude that there exists an integer <m>n</m> such that <m>n^2 + n - u = 0</m>.  Then,
    <me>
      u = n \left( n + 1 \right)
    </me>.
    From Exercise<nbsp/>(1), we know that <m>n(n + 1)</m> is even and hence, <m>u</m> is even.  This contradicts the assumption that <m>u</m> is odd.
  </ul>
  <ul>
    {{ <xref ref="exer_sec35-5"></xref>.}}
    \item If <m>n</m> is an odd integer, then there exists an integer <m>m</m> such that <m>n = 2m + 1</m>.  Use two cases: (1) <m>m</m> is even; (2) <m>m</m> is odd.  If <m>m</m> is even, then there exists an integer <m>k</m> such that <m>m = 2k</m> and this means that <m>n = 2(2k) + 1</m> or <m>n = 4k + 1</m>.  If <m>m</m> is odd, then there exists an integer <m>k</m> such that <m>m = 2k + 1</m>.  Then <m>n = 2(2k + 1) + 1</m> or <m>n = 4k + 3</m>.
  </ul>
  <ul>
    {{ <xref ref="exer_sec34-quadratic"></xref>.}}
    \item If <m>a \in \Z</m> and <m>a^2 = a</m>, then <m>a(a - 1) = 0</m>.  Since the product is equal to zero, at least one of the factors must be zero.  In the first case, <m>a = 0</m>.  In the second case,
    <m>a - 1 = 0</m> or <m>a = 1</m>.
  </ul>
  <ul>
    {{ <xref ref="exer_dividesproduct"></xref>.}}
    \item
    <ul>
      {{(c)}}
      \item For all integers  <m>a</m>, <m>b</m>, and  <m>d</m>  with <m>d \ne 0</m>, if  <m>d</m>  divides the product  <m>ab</m>, then <m>d</m>  divides  <m>a</m>  or  <m>d</m>  divides  <m>b</m>.
    </ul>
  </ul>
  <ul>
    {{ <xref ref="exer_sec34-6"></xref>.}}
    \item
    <ol>
      <li>
        <p>
          The statement, for all integers <m>m</m> and <m>n</m>,
          if 4 divides <m>\left(m^2 + n^2 - 1 \right)</m>,
          then <m>m</m> and <m>n</m> are consecutive integers, is false.
          A counterexample is <m>m = 2</m> and <m>n = 5</m>.
          The statement, for all integers <m>m</m> and <m>n</m>,
          if <m>m</m> and <m>n</m> are consecutive integers,
          then 4 divides <m>\left(m^2 + n^2 - 1 \right)</m>, is true.
          To prove this, let <m>n = m + 1</m>.
          Then
          <me>
            m^2 + n^2 - 1 = 2m^2 + 2m = 2m(m + 1)
          </me>.
          We have proven the <m>m(m + 1)</m> is even.  (See Exercise<nbsp/>(1).)  So this can be used to prove that 4 divides <m>\left(m^2 + n^2 - 1 \right)</m>.
        </p>
      </li>
    </ol>
  </ul>
  <ul>
    {{ <xref ref="exer_a2plus1not2n"></xref>.}}
    \item Try a proof by contradiction with two cases:  <m>a</m> is even or <m>a</m> is odd.
  </ul>
  <ul>
    {{ <xref ref="exer_absvalue"></xref>.}}
    \item
    <ul>
      {{(a)}}
      \item  One way is to use three cases:  (i) <m>x > 0</m>; (ii) <m>x = 0</m>; and <m>x \lt  0</m>.  For the first case, <m>-x \lt  0</m> and <m>\left| -x \right| = -( -x ) = x = \left| x \right|</m>.
    </ul>
  </ul>
  <ul>
    {{ <xref ref="exer_absvaluex"></xref>.}}
    \item
    <ul>
      {{(a)}}
      \item  For each real number <m>x</m>, <m>\left| x \right| \geq a</m> if and only if <m>x \geq a</m> or
      <m>x \leq -a</m>.
    </ul>
  </ul>
</section>