<section>
  <title><xref ref="S_compositionoffunctions"></xref></title>
  <ul>
    {{ <xref ref="exer64_notcommutative"></xref>.}}
    \item <m>( {g \circ h} ):\mathbb{R} \to \mathbb{R}</m>  by
    <m>( {g \circ h} )( x ) = g( {h( x )} ) = g\!\left( {x^3 } \right) = 3x^3  + 2</m>.
    <m>( {h \circ g} ):\mathbb{R} \to \mathbb{R}</m>  by
    <m>( {h \circ g} )( x ) = h( {g( x )} ) = h( {3x + 2} ) = ( {3x + 2} )^3</m>.
    This shows that <m>h \circ g \ne g \circ h</m> or that composition of functions is not commutative.
  </ul>
  <ul>
    {{ <xref ref="exer_sec64-2"></xref>.}}
    \item
    <ol>
      <li>
        <p>
          <m>F\left( x \right) = \left( {g \circ f} \right)\left( x \right)</m>,
          where <m>f\left( x \right) = e^x</m> and <m>g\left( x \right) = \cos x</m>.
        </p>
      </li>
      <li>
        <p>
          <m>G\left( x \right) = \left( {g \circ f} \right)\left( x \right)</m> where
          <m>f\left( x \right) = \cos x</m> and <m>g\left( x \right) = e^x</m>.
        </p>
      </li>
      <li>
        <p>
          <m>H\left( x \right) = \left( {g \circ f} \right)\left( x \right)</m>,
          <m>f\left( x \right) = \sin x</m>,
          <m>g\left( x \right) = \frac{1}{x}</m>.
        </p>
      </li>
      <li>
        <p>
          <m>K\left( x \right) = \left( {g \circ f} \right)\left( x \right)</m>,
          <m>f\left( x \right) = e^{-x^2}</m>,
          <m>g\left( x \right) = \cos x</m>.
        </p>
      </li>
    </ol>
  </ul>
  <ul>
    {{ <xref ref="exer_sec64-4"></xref>.}}
    \item
    <ul>
      {{(a)}}
      \item For each  <m>x \in A</m>, <m>( {f \circ I_A } )( x ) = f( {I_A ( x )} ) = f( x )</m>.  Therefore,
      <m>f \circ I_A  = f</m>.
    </ul>
  </ul>
  <ul>
    {{ <xref ref="exer_sec64-3"></xref>.}}
    \item
    <ul>
      {{(a)}}
      \item <m>\left[ {( {h \circ g} ) \circ f} \right]( x ) = \sqrt[3]{{\sin ( {x^2 } )}}</m>;
      <m>\left[ {h \circ ( {g \circ f} )} \right]( x ) = \sqrt[3]{{\sin ( {x^2 } )}}</m>.  This proves that <m>(h \circ g) \circ f = h \circ (g \circ f)</m> for these particular functions.
    </ul>
  </ul>
  <ul>
    {{ <xref ref="exer_sec64-5"></xref>.}}
    \item Start of a proof:  Let  <m>A</m>, <m>B</m>, and  <m>C</m>  be nonempty sets and let  <m>f\x A \to B</m>  and
    <m>g\x B \to C</m>.  Assume that
    <m>f</m>  and  <m>g</m>  are both injections.  Let  <m>x, y \in A</m> and assume that
    <m>( {g \circ f} )( x ) = ( {g \circ f} )( y )</m>.
  </ul>
  <ul>
    {{ <xref ref="exer_sec64-8"></xref>.}}
    \item
    <ul>
      {{(a)}}
      \item <m>f\x \mathbb{R} \to \mathbb{R}</m> by <m>f ( x ) = x</m>,
      <m>g: \mathbb{R} \to \mathbb{R}</m> by <m>g ( x ) = x^2</m>.  Then
      <m>g \circ f: \R \to \R</m> by <m>(g \circ f)(x) = x^2</m>.  The function <m>f</m> is a surjection, but <m>g \circ f</m> is not a surjection.
    </ul>
  </ul>
  <ul>
    \item
    <ul>
      {{(b)}}
      \item <m>f: \mathbb{R} \to \mathbb{R}</m> by <m>f \left( x \right) = x</m>,
      <m>g: \mathbb{R} \to \mathbb{R}</m> by <m>g \left( x \right) = x^2</m>.  Then
      <m>g \circ f: \R \to \R</m> by <m>(g \circ f)(x) = x^2</m>.  The function <m>f</m> is an injection, but <m>g \circ f</m> is not an injection.
    </ul>
  </ul>
  <ul>
    \item
    <ul>
      {{(f)}}
      \item By Part<nbsp/><xref ref="T_morecompositefunctions1"/> of <xref ref="T_morecompositefunctions">Theorem</xref>, this is not possible since if <m>g \circ f</m> is an injection, then <m>f</m> is an injection.
    </ul>
  </ul>
</section>