<section>
  <title><xref ref="S_functionsonsets"></xref></title>
  <ul>
    {{ <xref ref="exer_sec91-1"></xref>.}}
    \item
    <ul>
      {{(a)}}
      \item There exists an <m>x \in A \cap B</m> such that <m>f ( x ) = y</m>.
    </ul>
  </ul>
  <ul>
    \item
    <ul>
      {{(d)}}
      \item There exists an <m>a \in A</m> such that <m>f ( a ) = y</m> or there exists a
      <m>b \in B</m> such that <m>f ( b ) = y</m>.
    </ul>
  </ul>
  <ul>
    \item
    <ul>
      {{(f)}}
      \item <m>f ( x ) \in C \cup D</m>
    </ul>
  </ul>
  <ul>
    \item
    <ul>
      {{(h)}}
      \item <m>f ( x ) \in C</m> or <m>f ( x ) \in D</m>
    </ul>
  </ul>
  <ul>
    {{ <xref ref="exer_sec91-2"></xref>.}}
    \item
    <ul>
      {{(b)}}
      \item <m>f^{-1} \left( f ( A ) \right) = \left[ 2, 5 \right]</m>.
    </ul>
  </ul>
  <ul>
    \item
    <ul>
      {{(d)}}
      \item <m>f ( f^{-1} ( C ) ) = \left[ -2, 3 \right]</m>
    </ul>
  </ul>
  <ul>
    \item
    <ul>
      {{(e)}}
      \item <m>f ( A \cap B ) = \left[ -5, -3 \right]</m>
    </ul>
  </ul>
  <ul>
    \item
    <ul>
      {{(f)}}
      \item <m>f ( A ) \cap f ( B ) = \left[ -5, -3 \right]</m>
    </ul>
  </ul>
  <ul>
    {{ <xref ref="exer_sec91-3"></xref>.}}
    \item
    <ul>
      {{(a)}}
      \item <m>g ( A \times A ) = \left\{6, 12, 18, 24, 36, 54, 72, 108, 216 \right\}</m>
    </ul>
  </ul>
  <ul>
    \item
    <ul>
      {{(b)}}
      \item <m>g^{-1} ( C ) = \left\{ ( 1, 1 ), ( 2, 1 ),
      ( 1, 2 ) \right\}</m>
    </ul>
  </ul>
  <ul>
    {{ <xref ref="exer_sec91-4"></xref>.}}
    \item
    <ul>
      {{(a)}}
      \item <m>\text{ range }  ( F ) = F ( S ) = \left\{1, 4, 9, 16 \right\}</m>
    </ul>
  </ul>
  <ul>
    {{ <xref ref="exer_sec91-5"></xref>.}}
    \item To prove <m>f \left( A \cup B \right) \subseteq f \left( A \right) \cup f \left( B \right)</m>, let <m>y \in f \left( A \cup B \right)</m>.  Then there exists an <m>x \in A \cup B</m> such that <m>f \left( x \right) = y</m>.  Since <m>x \in A \cup B</m>, <m>x \in A</m> or <m>x \in B</m>.  We first note that if <m>x \in A</m>, then <m>y = f \left( x \right)</m> is in <m>f \left( A \right)</m>.  In addition, if <m>x \in B</m>, then <m>y = f \left( x \right)</m> is in <m>f \left( B \right)</m>.
    In both cases, <m>y = f \left( x \right) \in f \left( A \right) \cup f \left( B \right)</m> and hence,
    <m>f \left( A \cup B \right) \subseteq f \left( A \right) \cup f \left( B \right)</m>.
    Now let <m>y \in f \left( A \right) \cup f \left( B \right)</m>.  If <m>y \in f \left( A \right)</m>, then there exists an <m>x \in A</m> such that <m>y = f \left( x \right)</m>.  Since <m>A \subseteq A \cup B</m>, this implies that <m>y = f \left( x \right) \in f \left( A \cup B \right)</m>.  In a similar manner, we can prove that if <m>y \in f \left( B \right)</m>, then <m>y \in f \left( A \cup B \right)</m>.  Therefore,
    <m>f \left( A \right) \cup f \left( B \right) \subseteq f \left( A \cup B \right)</m>.
  </ul>
  <ul>
    {{ <xref ref="exer_sec91-6"></xref>.}}
    \item To prove that
    <m>f^{-1} ( C \cap D ) \subseteq f^{-1} ( C ) \cap f^{-1} ( D )</m>, let <m>x \in f^{-1} ( C \cap D )</m>.  Then <m>f(x) \in C \cap D</m>.  How do we prove that
    <m>x \in f^{-1} ( C ) \cap f^{-1} ( D )</m>?
  </ul>
  <ul>
    {{ <xref ref="exer_invimagetruefalse"></xref>.}}
    \item Statement (a) is true and Statement (b) is false.
  </ul>
</section>